Refinery/Ctx/Semantics.lean
@@ -11,6 +11,8 @@ open MonoidalCategory
 
 open Monoidal
 
+open EffectfulCategory
+
 section TyModel
 
 variable {α : Type _} [HasQuant α]
@@ -43,21 +45,21 @@ def Var?.Wk.den {v w : Var? α ε} (h : v ≤ w) : (v⟦ v ⟧ : C) ⟶ v⟦ w �
   | v, ⟨B, 0, _⟩, h => (h.unused_del rfl).den
   | ⟨A, (_ : Quant), _⟩, ⟨B, (_ : Quant), _⟩, h => eq_hom (by cases h.ty; rfl)
 
+@[simp]
+theorem Var?.Wk.den_zero {v : Var? α ε} {A : Ty α} {e : ε} (h : v ≤ ⟨A, 0, e⟩)
+  : Var?.Wk.den (C := C) h = (h.unused_del rfl).den
+  := by cases v with | mk _ q _ => cases q <;> rfl
+
+@[simp]
+theorem Var?.Wk.den_quant {v : Var? α ε} {A : Ty α} {q : Quant} {e : ε} (h : v ≤ ⟨A, q, e⟩)
+  : Var?.Wk.den (C := C) h = eq_hom (by rw [ety_eq_quant h])
+  := by cases v with | mk _ q' _ =>
+        cases q' with | zero => have h := h.q; cases h using EQuant.le.casesLE | _ => rfl
+
 def Ctx?.PWk.den {Γ Δ : Ctx? α ε} (h : Γ.PWk Δ) : (g⟦ Γ ⟧ : C) ⟶ g⟦ Δ ⟧
   := match Γ, Δ, h with
   | .nil, .nil, _ => 𝟙 (𝟙_ C)
   | .cons _ _, .cons _ _, h => h.tail.den ⊗ (Var?.Wk.den h.head)
-
-def Var?.PSSplit.den {u v w : Var? α ε} : u.PSSplit v w → ((v⟦ u ⟧ : C) ⟶ v⟦ v ⟧ ⊗ v⟦ w ⟧)
-  | .left _ _ _ => (ρ_ _).inv
-  | .right _ _ _ => (λ_ _).inv
-  | .sboth h => have _ := h.copy; Δ_ _
-
-variable [BraidedCategoryStruct C]
-
-def Ctx?.PSSplit.den {Γ Δ Ξ : Ctx? α ε} : Γ.PSSplit Δ Ξ → ((g⟦ Γ ⟧ : C) ⟶ g⟦ Δ ⟧ ⊗ g⟦ Ξ ⟧)
-  | .nil => (λ_ _).inv
-  | .cons hΓ hv => (hΓ.den ⊗ hv.den) ≫ swap_inner _ _ _ _
 
 def Ctx?.Wk.den {Γ Δ : Ctx? α ε} : Γ.Wk Δ → ((g⟦ Γ ⟧ : C) ⟶ g⟦ Δ ⟧)
   | .nil => 𝟙 (𝟙_ C)
@@ -72,6 +74,118 @@ def Ctx?.At.den {v : Var? α ε} {Γ : Ctx? α ε} {n} (h : Γ.At v n) : (g⟦ �
     (λ _ d _ h => (d.den ⊗ (Var?.Wk.den h)) ≫ (λ_ _).hom)
     (λ _ _ _ _ hw p => (p ⊗ hw.den) ≫ (ρ_ _).hom)
 
+@[simp]
+theorem Ctx?.At.den_zero {v w : Var? α ε} {Γ : Ctx? α ε} (h : (Γ.cons w).At v 0)
+  : h.den (C := C)
+  = (h.zero_cons_tail.den (C := C) ⊗ (Var?.Wk.den h.zero_cons_head)) ≫ (λ_ _).hom
+  := rfl
+
+@[simp]
+theorem Ctx?.At.den_succ {v w : Var? α ε} {Γ : Ctx? α ε} (h : (Γ.cons w).At v (n + 1))
+  : h.den (C := C)
+  = (h.succ_cons_tail.den (C := C) ⊗ h.succ_cons_head.den) ≫ (ρ_ _).hom
+  := rfl
+
+def Var?.PSSplit.den {u v w : Var? α ε} : u.PSSplit v w → ((v⟦ u ⟧ : C) ⟶ v⟦ v ⟧ ⊗ v⟦ w ⟧)
+  | .left _ _ _ => (ρ_ _).inv
+  | .right _ _ _ => (λ_ _).inv
+  | .sboth h => have _ := h.copy; Δ_ _
+
+theorem Var?.Wk.den_eff_in {v : Var? α ε} {A : Ty α} {q} {e e' : ε}
+  (h : v ≤ ⟨A, q, e⟩) (h' : v ≤ ⟨A, q, e'⟩)
+  : Var?.Wk.den (C := C) h = Var?.Wk.den h'
+  := by cases q using EQuant.casesZero <;> simp
+
+theorem Ctx?.At.den_eff {A : Ty α} {q} {e e' : ε} {Γ : Ctx? α ε} {n}
+  (hΓe : Γ.At ⟨A, q, e⟩ n) (hΓe' : Γ.At ⟨A, q, e'⟩ n)
+  : hΓe.den (C := C) = hΓe'.den
+  := by induction hΓe with
+  | here =>
+    cases hΓe'; simp only [den_zero, Iso.cancel_iso_hom_right]; congr 1; apply Var?.Wk.den_eff_in
+  | there _ _ _ _ _ I => cases hΓe'; simp [*]
+
+variable [BraidedCategoryStruct C]
+
+def Ctx?.PSSplit.den {Γ Δ Ξ : Ctx? α ε} : Γ.PSSplit Δ Ξ → ((g⟦ Γ ⟧ : C) ⟶ g⟦ Δ ⟧ ⊗ g⟦ Ξ ⟧)
+  | .nil => (λ_ _).inv
+  | .cons hΓ hv => (hΓ.den ⊗ hv.den) ≫ swap_inner _ _ _ _
+
+end VarModel
+
+variable {φ : Type _} {α : Type _} {ε : Type _} [Signature φ α ε]
+         {C : Type _} [Category C] [MonoidalCategoryStruct C] [ChosenFiniteCoproducts C]
+         [BraidedCategoryStruct C] [Iterate C] [E : Elgot2 C ε]
+         [M : Model φ α ε C]
+
+@[simp]
+theorem Var?.Wk.den_eff {A : Ty α} {q : EQuant} {e e' : ε} (h : ⟨A, q, e⟩ ≤ ⟨A, q, e'⟩)
+  : Var?.Wk.den (C := C) h = 𝟙 _
+  := by cases q using EQuant.casesZero with
+    | zero => simp [Var?.del.den, ety]; rfl
+    | rest q => rfl
+
+@[simp]
+theorem Var?.del.den_pure {v : Var? α ε} (h : v.del) : E.HasEff e h.den := inferInstance
+
+@[simp]
+theorem Var?.copy.den_pure {v : Var? α ε} (h : v.copy) : E.HasEff e h.den := inferInstance
+
+@[simp]
+instance Var?.Wk.den_pure {e : ε} {v w : Var? α ε} (h : v ≤ w)
+  : E.HasEff e <| Var?.Wk.den h
+  := by cases v with | mk _ qv _ => cases w with | mk _ qw _ => cases qw using EQuant.casesZero with
+    | zero => rw [den_zero]; infer_instance
+    | rest qw => rw [den_quant]; infer_instance
+
+instance Var?.Wk.den_central {v w : Var? α ε} (h : v ≤ w)
+  : Central (C := C) (Var?.Wk.den h)
+  := (den_pure h).pure_central
+
+theorem Var?.Wk.den_comp {u v w : Var? α ε} (h : u ≤ v) (h' : v ≤ w)
+  : den h ≫ den h' = den (C := C) (le_trans h h')
+  := by cases u with | mk _ qu _ => cases v with | mk _ qv _ => cases w with | mk _ qw _ =>
+    cases qw using EQuant.casesZero with
+    | zero =>
+      simp [Var?.del.den]
+      exact M.drop_aff (⊥ : ε) _ (hA := ety_aff_zero (le_trans h h')) (hB := ety_aff_zero h')
+    | rest qw =>  cases qv using EQuant.casesZero with
+    | zero => cases h'.q using EQuant.le.casesLE
+    | rest qv => simp
+
+variable [IsPremonoidal C]
+
+instance Ctx?.Wk.den_pure {Γ Δ : Ctx? α ε} (h : Γ.Wk Δ) : E.HasEff e h.den := by induction h with
+  | nil => simp only [den]; exact HasEff.id
+  | skip =>
+    simp only [den]; apply HasEff.comp (hf := _) (hg := _); apply HasEff.tensorHom; infer_instance
+  | cons => simp only [den]; infer_instance
+
+instance Ctx?.Wk.den_central {Γ Δ : Ctx? α ε} (h : Γ.Wk Δ) : Central (C := C) h.den
+  := (den_pure h).pure_central
+
+instance Ctx?.At.den_pure {v : Var? α ε} {Γ : Ctx? α ε} {n} (h : Γ.At v n)
+  : E.HasEff e h.den
+  := by induction h <;> simp <;> infer_instance
+
+instance Ctx?.At.den_central {v : Var? α ε} {Γ : Ctx? α ε} {n} (h : Γ.At v n)
+  : Central (C := C) h.den
+  := (den_pure h).pure_central
+
+@[simp]
+theorem Ctx?.At.den_wkOut {v w : Var? α ε} {Γ : Ctx? α ε} {n} (hΓv : Γ.At v n) (hvw : v ≤ w)
+  : hΓv.den (C := C) ≫ Var?.Wk.den hvw = (hΓv.wkOut hvw).den
+  := by induction hΓv with
+  | here =>
+    simp only [Ctx?.den, ety, Ty.den, den_zero, Monoidal.tensorHom_def, Category.assoc, ←
+      Monoidal.leftUnitor_naturality]
+    rw [<-Monoidal.whiskerLeft_comp_assoc, Var?.Wk.den_comp]
+    rfl
+  | there _ _ _ _ _ I =>
+    simp only [den_succ, Category.assoc, ← Monoidal.rightUnitor_naturality]
+    rw [Monoidal.tensor_eq_rtimes_left, Monoidal.tensor_eq_rtimes_left]
+    simp only [rtimes, Category.assoc]
+    rw [<-Monoidal.whiskerRight_comp_assoc, I]
+
 -- TODO: Ctx?.At.ix.den = Ctx?.At.den
 
 -- TODO: Var?.Ix.at.den = Var?.Ix.den
@@ -85,5 +199,3 @@ def Ctx?.At.den {v : Var? α ε} {Γ : Ctx? α ε} {n} (h : Γ.At v n) : (g⟦ �
 -- TODO: PSSplit ==> PSSplit, PSSplit vs PSSplit?
 
 -- TODO: Split? SSplit?
-
-end VarModel
