Refinery/Model.lean
@@ -83,27 +83,51 @@ class Model
   copy_unit : copy .unit = (λ_ _).inv
   copy_tensor {A B} [IsRel A] [IsRel B]
     : copy (.tensor A B) = (copy A ⊗ copy B) ≫ swap_inner _ _ _ _
-  drop_rem {A B : Ty α} {e : ε} (f : t⟦ A ⟧ ⟶ t⟦ B ⟧) (h : E.eff e f)
+  drop_rem {A B : Ty α} (e : ε) (f : t⟦ A ⟧ ⟶ t⟦ B ⟧) [h : E.HasEff e f]
     [IsAff A] [IsAff B] [hf : IsRem e] : f ≫ drop _ ↠ drop _
-  copy_drop_left_rem {A B : Ty α} {e : ε} (f : t⟦ A ⟧ ⟶ t⟦ B ⟧) (h : E.eff e f)
+  copy_drop_left_rem {A B : Ty α} (e : ε) (f : t⟦ A ⟧ ⟶ t⟦ B ⟧) [h : E.HasEff e f]
     [IsRel A] [IsAff B] [hf : IsRem e] : copy _ ≫ (f ≫ drop _) ▷ t⟦ A ⟧ ↠ (λ_ _).inv
-  copy_dup_ltimes {A B : Ty α} {e : ε} (f : t⟦ A ⟧ ⟶ t⟦ B ⟧) (h : E.eff e f)
+  copy_dup_ltimes {A B : Ty α} (e : ε) (f : t⟦ A ⟧ ⟶ t⟦ B ⟧) [h : E.HasEff e f]
     [IsRel A] [IsRel B] [hf : IsDup e] : f ≫ copy _ ↠ copy _ ≫ (f ⋉ f)
-  copy_dup_rtimes {A B : Ty α} {e : ε} (f : t⟦ A ⟧ ⟶ t⟦ B ⟧) (h : E.eff e f)
+  copy_dup_rtimes {A B : Ty α} (e : ε) (f : t⟦ A ⟧ ⟶ t⟦ B ⟧) [h : E.HasEff e f]
     [IsRel A] [IsRel B] [hf : IsDup e] : f ≫ copy _ ↠ copy _ ≫ (f ⋊ f)
-  drop_add {A B : Ty α} {e : ε} (f : t⟦ A ⟧ ⟶ t⟦ B ⟧) (h : E.eff e f)
+  drop_add {A B : Ty α} (e : ε) (f : t⟦ A ⟧ ⟶ t⟦ B ⟧) [h : E.HasEff e f]
     [IsAff A] [IsAff B] [hf : IsAdd e] : f ≫ drop _ ↞ drop _
-  copy_drop_left_add {A B : Ty α} {e : ε} (f : t⟦ A ⟧ ⟶ t⟦ B ⟧) (h : E.eff e f)
+  copy_drop_left_add {A B : Ty α} (e : ε) (f : t⟦ A ⟧ ⟶ t⟦ B ⟧) [h : E.HasEff e f]
     [IsRel A] [IsAff B] [hf : IsAdd e] : copy _ ≫ (f ≫ drop _) ▷ t⟦ A ⟧ ↞ (λ_ _).inv
-  copy_fuse_ltimes {A B : Ty α} {e : ε} (f : t⟦ A ⟧ ⟶ t⟦ B ⟧) (h : E.eff e f)
+  copy_fuse_ltimes {A B : Ty α} (e : ε) (f : t⟦ A ⟧ ⟶ t⟦ B ⟧) [h : E.HasEff e f]
     [IsRel A] [IsRel B] [hf : IsFuse e] : f ≫ copy _ ↞ copy _ ≫ (f ⋉ f)
-  copy_fuse_rtimes {A B : Ty α} {e : ε} (f : t⟦ A ⟧ ⟶ t⟦ B ⟧) (h : E.eff e f)
+  copy_fuse_rtimes {A B : Ty α} (e : ε) (f : t⟦ A ⟧ ⟶ t⟦ B ⟧) [h : E.HasEff e f]
     [IsRel A] [IsRel B] [hf : IsFuse e] : f ≫ copy _ ↞ copy _ ≫ (f ⋊ f)
 
-variable [Iterate C] [E : Elgot2 C ε] [Model φ α ε C]
+attribute [simp] Model.drop_unit Model.copy_unit
+
+variable [Iterate C] [E : Elgot2 C ε] [M : Model φ α ε C]
+
+theorem Model.drop_aff {A B : Ty α} (e : ε) (f : t⟦ A ⟧ ⟶ t⟦ B ⟧) [h : E.HasEff e f]
+    [hA : IsAff A] [hB : IsAff B] [hf : IsAff e] : f ≫ !_ _ = !_ _
+    := refines_antisymm (drop_rem e f) (drop_add e f)
+
+theorem Model.copy_drop_left {A B : Ty α} (e : ε) (f : t⟦ A ⟧ ⟶ t⟦ B ⟧) [h : E.HasEff e f]
+    [hA : IsRel A] [hB : IsAff B] [hf : IsAff e] : Δ_ _ ≫ (f ≫ !_ _) ▷ t⟦ A ⟧ = (λ_ _).inv
+    := refines_antisymm (copy_drop_left_rem e f) (copy_drop_left_add e f)
+
+theorem Model.copy_rel_ltimes {A B : Ty α} (e : ε) (f : t⟦ A ⟧ ⟶ t⟦ B ⟧) [h : E.HasEff e f]
+    [hA : IsRel A] [hB : IsRel B] [hf : IsRel e] : f ≫ Δ_ _ = Δ_ _ ≫ (f ⋉ f)
+    := refines_antisymm (copy_dup_ltimes e f) (copy_fuse_ltimes e f)
+
+theorem Model.copy_rel_rtimes {A B : Ty α} (e : ε) (f : t⟦ A ⟧ ⟶ t⟦ B ⟧) [h : E.HasEff e f]
+    [hA : IsRel A] [hB : IsRel B] [hf : IsRel e] : f ≫ Δ_ _ = Δ_ _ ≫ (f ⋊ f)
+    := refines_antisymm (copy_dup_rtimes e f) (copy_fuse_rtimes e f)
 
 instance Model.dropCentral {A : Ty α} [IsAff A] : Central (C := C) (!_ A)
   := E.pure_hom_central drop_pure
 
 instance Model.copyCentral {A : Ty α} [IsRel A] : Central (C := C) (Δ_ A)
   := E.pure_hom_central copy_pure
+
+instance Model.drop_eff {e : ε} {A : Ty α} [IsAff A] : E.HasEff e (!_ A) where
+  has_eff := E.eff.monotone' bot_le _ M.drop_pure
+
+instance Model.copy_eff {e : ε} {A : Ty α} [IsRel A] : E.HasEff e (Δ_ A) where
+  has_eff := E.eff.monotone' bot_le _ M.copy_pure
