Refinery/Term/Extrinsic/Semantics.lean
@@ -17,25 +17,6 @@ variable {φ : Type _} {α : outParam (Type _)} {ε : outParam (Type _)} [S : Si
 
 namespace Term
 
-def Wf.den {Γ : Ctx? α ε} {A : Ty α} {a : Term φ} : (Γ ⊢ a : A) → ((g⟦ Γ ⟧ : C) ⟶ t⟦ A ⟧)
-  | .bv hv => hv.den
-  | .op hf da => da.den ≫ hf.den
-  | .let₁ dΓ da db => dΓ.den ≫ (_ ◁ da.den) ≫ db.den
-  | .unit dΓ => dΓ.den
-  | .pair dΓ da db => dΓ.den ≫ (da.den ⋉ db.den)
-  | .let₂ dΓ da db => dΓ.den ≫ (_ ◁ da.den) ≫ (α_ _ _ _).inv ≫ db.den
-  | .inl da => da.den ≫ CC.inl _ _
-  | .inr db => db.den ≫ CC.inr _ _
-  | .case dΓ da db dc => dΓ.den ≫ (_ ◁ da.den) ≫ (∂L _ _ _).inv ≫ desc db.den dc.den
-  | .abort da => da.den ≫ CC.fromZero _
-  | .iter (A := A) (B := B) (Γr := Γr) dΓ _ _ da db =>
-    dΓ.den ≫ (_ ◁ da.den) ≫ iterate (
-      Δ_ Γr.ety ▷ _
-        ≫ (α_ _ _ _).hom
-        ≫ _ ◁ db.den
-        ≫ (∂L g⟦Γr⟧ t⟦B⟧ t⟦A⟧).inv
-        ≫ ((!_ Γr.ety ▷ _ ≫ (λ_ _).hom) ⊕ₕ 𝟙 _))
-
 def Deriv.den {e : ε} {Γ : Ctx? α ε} {A : Ty α} {a : Term φ}
   : (Γ ⊢[e] a : A) → ((g⟦ Γ ⟧ : C) ⟶ t⟦ A ⟧)
   | .bv hv => hv.den
@@ -56,6 +37,9 @@ def Deriv.den {e : ε} {Γ : Ctx? α ε} {A : Ty α} {a : Term φ}
         ≫ (∂L g⟦Γr⟧ t⟦B⟧ t⟦A⟧).inv
         ≫ ((!_ Γr.ety ▷ _ ≫ (λ_ _).hom) ⊕ₕ 𝟙 _))
 
-theorem Deriv.den_toWf {e : ε} {Γ : Ctx? α ε} {A : Ty α} {a : Term φ}
-  (D : Γ ⊢[e] a : A) : D.toWf.den = D.den (C := C)
-  := by induction D <;> simp only [toWf, den, Wf.den, *]
+@[simp]
+theorem Deriv.den_mono {e e' : ε} {Γ : Ctx? α ε} {A : Ty α} {a : Term φ}
+  (he : e ≤ e') (D : Γ ⊢[e] a : A) : (D.mono he).den = D.den (C := C)
+  := by induction D with
+  | bv => simp only [den, mono]; rw [Ctx?.At.den_eff]
+  | _ => simp only [den, mono, *] <;> rfl
